# Product Rule for Derivatives

Created: 2018-12-05 00:20:24 +0500

Modified: 2018-12-05 00:33:06 +0500

---

![The Product Rule Suppose f (x) and g(x) are functions. There are 5 fundamental function operations: + --- For each operation there is a derivative rule: x O f (x) + g(x) 2. f (x) --- g(x) 4. Sum Rule Difference Rule Product Rule Quotient Rule Chain Rule' ](media/Product-Rule-for-Derivatives-image1.png){width="5.0in" height="3.0833333333333335in"}

Fifth is *function composition*
![1. Sum Rule: 2. Difference Rule: 3. Product Rule: 4. Quotient Rule: 5. Chain Rule: f' (x) • g(x) + f (x) • g' (x) [ LIE.)] ' --- --- (x) [ g(x) 12 [f 0 g(x) ] ' = f' (g(x)) •g' (x) ](media/Product-Rule-for-Derivatives-image2.png){width="5.0in" height="1.4895833333333333in"}
3.  Product Rule

![Let f (x) and g(x) be two functions. Question: What is the derivative of f (x) • g(x) ? It's common to leave out the x's: There are other ways to write the derivative: dx•g+fÆ dx f' (x) can be written as dx • ](media/Product-Rule-for-Derivatives-image3.png){width="5.0in" height="1.78125in"}
![Example Find the derivative of (x2 --- 2) (7 x3 + 5). There are two ways to do this: 1. Multiply the two polynomials, then take the derivative 2. Use the product rule l. Multiply, then differentiate: (x2 -2) - +5x2- 10 Derivative of (x2 --- 2) (7 x3 + 5) is 35 x4 --- 42x2 + 10 x. ](media/Product-Rule-for-Derivatives-image4.png){width="5.0in" height="2.5520833333333335in"}
![2. Use the product rule: t t g(x) g (x) = 7 5 (x) = 21 = 14 X4+ 42 X2 =35x4-42x2+10x - 2) (21 x2) ](media/Product-Rule-for-Derivatives-image5.png){width="5.0in" height="2.1354166666666665in"}
![Caution Common mistake: [f = f' •g' Tip: Write down what you think is the formula, then test it! Test: Let f (x) = x2 and g(x) = x3 f (x) • g(x) = x2 • x3 = x5 [x5]' --- 5x4 Now test the formula: (2 x) • (3 x2) = 6 x3 * 5 x4 This formula is wrong! ](media/Product-Rule-for-Derivatives-image6.png){width="5.0in" height="3.1354166666666665in"}
![Generalizations Find the derivative of 17 x • cos x • ex. This function is the product of three functions, not two: (17 x) (cos x) (ex). Trick: Use the product rule repeatedly. - + (f.g).h' ](media/Product-Rule-for-Derivatives-image7.png){width="5.0in" height="2.6770833333333335in"}
![Example Find the derivative of 17 x • cos x • ex. This is the product of 3 functions which we know how to differentiate: (17 X) (COS X) (ex ) Let f (x) = 17 x, g(x) = cos x, and h(x) = ex. = (17) (COS X) (ex ) + (17 X) (---sin X) (ex ) + (17 X) (COS X) (ex) --- 17 cosx•ex--- 17 x •sinx•eX+ 17 ](media/Product-Rule-for-Derivatives-image8.png){width="5.0in" height="2.1354166666666665in"}
**References**

[Product Rule for Derivatives (Calculus)](https://www.youtube.com/watch?v=8Qw2aPjqW9c)
![The Product Rule ](media/Product-Rule-for-Derivatives-image9.jpg){width="5.0in" height="2.8020833333333335in"}
